

# Four-valued logics of indicative conditionals

M. Muñoz Pérez

Universidad Nacional de Educación a Distancia (UNED)  
Madrid, Spain

ReacTS Workshop 2025  
Toledo, November 11, 2025



# 1. Formalizing indicative conditionals

# 1. Formalizing indicative conditionals

What are indicative conditionals?

# 1. Formalizing indicative conditionals

What are indicative conditionals? The simplest sentences of the *if-then* type that occur in natural language and are concerned with what could be true.

# 1. Formalizing indicative conditionals

What are indicative conditionals? The simplest sentences of the *if-then* type that occur in natural language and are concerned with what could be true.

**Example:** if Lee Harvey-Oswald didn't shoot JFK, someone else did.

# 1. Formalizing indicative conditionals

What are indicative conditionals? The simplest sentences of the *if-then* type that occur in natural language and are concerned with what could be true.

**Example:** if Lee Harvey-Oswald didn't shoot JFK, someone else did.

**Non-example:** if Lee Harvey-Oswald had not shot JFK, someone else would have.

# 1. Formalizing indicative conditionals

What are indicative conditionals? The simplest sentences of the *if-then* type that occur in natural language and are concerned with what could be true.

**Example:** if Lee Harvey-Oswald didn't shoot JFK, someone else did.

**Non-example:** if Lee Harvey-Oswald had not shot JFK, someone else would have.

Hence, one ought to distinguish between indicative conditionals and counterfactuals.

# 1. Formalizing indicative conditionals

What are indicative conditionals? The simplest sentences of the *if-then* type that occur in natural language and are concerned with what could be true.

**Example:** if Lee Harvey-Oswald didn't shoot JFK, someone else did.

**Non-example:** if Lee Harvey-Oswald had not shot JFK, someone else would have.

Hence, one ought to distinguish between indicative conditionals and counterfactuals.

We will denote the indicative conditional statement 'if  $\varphi$  then  $\psi$ ' by  $\varphi \rightarrow \psi$ .



# 1. Formalizing indicative conditionals

# 1. Formalizing indicative conditionals

Classical formalization: the indicative conditional  $\varphi \rightarrow \psi$  collapses to material implication  $\varphi \supset \psi$  ( $\sim \neg\varphi \vee \psi$ ).

# 1. Formalizing indicative conditionals

Classical formalization: the indicative conditional  $\varphi \rightarrow \psi$  collapses to material implication  $\varphi \supset \psi$  ( $\sim \neg\varphi \vee \psi$ ).

Strange behavior of  $\mathbf{0} \rightarrow x \dots$

# 1. Formalizing indicative conditionals

Classical formalization: the indicative conditional  $\varphi \rightarrow \psi$  collapses to material implication  $\varphi \supset \psi$  ( $\sim \neg\varphi \vee \psi$ ).

Strange behavior of  $\mathbf{0} \rightarrow x \dots$  is it a 'truth-value gap'? (Quine)

# 1. Formalizing indicative conditionals

Classical formalization: the indicative conditional  $\varphi \rightarrow \psi$  collapses to material implication  $\varphi \supset \psi$  ( $\sim \neg\varphi \vee \psi$ ).

Strange behavior of  $\mathbf{0} \rightarrow x \dots$  is it a 'truth-value gap'? (Quine)

**Solution:** add a new truth-value  $\frac{1}{2}$ !

# 1. Formalizing indicative conditionals

Classical formalization: the indicative conditional  $\varphi \rightarrow \psi$  collapses to material implication  $\varphi \supset \psi$  ( $\sim \neg\varphi \vee \psi$ ).

Strange behavior of  $\mathbf{0} \rightarrow x \dots$  is it a 'truth-value gap'? (Quine)

**Solution:** add a new truth-value  $\frac{1}{2}$ !

But what about  $\frac{1}{2} \rightarrow x$ ?

# 1. Formalizing indicative conditionals

Classical formalization: the indicative conditional  $\varphi \rightarrow \psi$  collapses to material implication  $\varphi \supset \psi$  ( $\sim \neg\varphi \vee \psi$ ).

Strange behavior of  $\mathbf{0} \rightarrow x \dots$  is it a 'truth-value gap'? (Quine)

**Solution:** add a new truth-value  $\frac{1}{2}$ !

But what about  $\frac{1}{2} \rightarrow x$ ?

Here, the intuitions may differ...

## 2. The three-valued case



## 2. The three-valued case

	$\neg$	$\rightarrow_{DF}$	<b>0</b>	$1/2$	<b>1</b>	$\rightarrow_{OL}$	<b>0</b>	$1/2$	<b>1</b>	$\rightarrow_F$	<b>0</b>	$1/2$	<b>1</b>
<b>0</b>	<b>1</b>	<b>0</b>	$1/2$	$1/2$	$1/2$	<b>0</b>	$1/2$	$1/2$	$1/2$	<b>0</b>	$1/2$	$1/2$	$1/2$
$1/2$	$1/2$	$1/2$	$1/2$	$1/2$	$1/2$	$1/2$	<b>0</b>	$1/2$	<b>1</b>	$1/2$	<b>0</b>	$1/2$	$1/2$
<b>1</b>	<b>0</b>	<b>1</b>	<b>0</b>	$1/2$	<b>1</b>	<b>1</b>	<b>0</b>	$1/2$	<b>1</b>	<b>1</b>	<b>0</b>	$1/2$	<b>1</b>

## 2. The three-valued case

	$\neg$	$\rightarrow_{DF}$	<b>0</b>	$\frac{1}{2}$	<b>1</b>	$\rightarrow_{OL}$	<b>0</b>	$\frac{1}{2}$	<b>1</b>	$\rightarrow_F$	<b>0</b>	$\frac{1}{2}$	<b>1</b>
<b>0</b>	<b>1</b>	<b>0</b>	$\frac{1}{2}$	$\frac{1}{2}$	$\frac{1}{2}$	<b>0</b>	$\frac{1}{2}$	$\frac{1}{2}$	$\frac{1}{2}$	<b>0</b>	$\frac{1}{2}$	$\frac{1}{2}$	$\frac{1}{2}$
$\frac{1}{2}$	$\frac{1}{2}$	$\frac{1}{2}$	$\frac{1}{2}$	$\frac{1}{2}$	$\frac{1}{2}$	$\frac{1}{2}$	<b>0</b>	$\frac{1}{2}$	<b>1</b>	$\frac{1}{2}$	<b>0</b>	$\frac{1}{2}$	$\frac{1}{2}$
<b>1</b>	<b>0</b>	<b>1</b>	<b>0</b>	$\frac{1}{2}$	<b>1</b>	<b>1</b>	<b>0</b>	$\frac{1}{2}$	<b>1</b>	<b>1</b>	<b>0</b>	$\frac{1}{2}$	<b>1</b>

$\wedge_K$	0	1/2	1
0	0	0	0
1/2	0	1/2	1/2
1	0	1/2	1

$\vee_K$	0	1/2	1
0	0	1/2	1
1/2	1/2	1/2	1
1	1	1	1

$\wedge_{OL}$	0	1/2	1
0	0	0	0
1/2	0	1/2	1
1	0	1	1

$\vee_{OL}$	0	1/2	1
0	0	0	1
1/2	0	1/2	1
1	1	1	1

## 2. The three-valued case

## 2. The three-valued case

Let  $A_3 := \{\mathbf{0}, \mathbf{1}/2, \mathbf{1}\}$ . Our three-valued logics are:

## 2. The three-valued case

Let  $A_3 := \{\mathbf{0}, \mathbf{1}/2, \mathbf{1}\}$ . Our three-valued logics are:

- *De Finetti's logic*  $\mathbf{DF}$ , induced by  $\langle \mathbf{DF}_3, \{\mathbf{1}/2, \mathbf{1}\} \rangle$ , with  $\mathbf{DF}_3 := \langle A_3; \neg, \wedge_K, \vee_K, \rightarrow_{\mathbf{DF}} \rangle$ .

## 2. The three-valued case

Let  $A_3 := \{0, 1/2, 1\}$ . Our three-valued logics are:

- *De Finetti's logic* DF, induced by  $\langle \mathbf{DF}_3, \{1/2, 1\} \rangle$ , with  $\mathbf{DF}_3 := \langle A_3; \neg, \wedge_K, \vee_K, \rightarrow_{DF} \rangle$ .
- *Cooper's logic* OL, induced by  $\langle \mathbf{OL}_3, \{1/2, 1\} \rangle$ , with  $\mathbf{OL}_3 := \langle A_3; \neg, \wedge_{OL}, \vee_{OL}, \rightarrow_{OL} \rangle$ .

## 2. The three-valued case

Let  $A_3 := \{0, 1/2, 1\}$ . Our three-valued logics are:

- *De Finetti's logic*  $DF$ , induced by  $\langle \mathbf{DF}_3, \{1/2, 1\} \rangle$ , with  $\mathbf{DF}_3 := \langle A_3; \neg, \wedge_K, \vee_K, \rightarrow_{DF} \rangle$ .
- *Cooper's logic*  $OL$ , induced by  $\langle \mathbf{OL}_3, \{1/2, 1\} \rangle$ , with  $\mathbf{OL}_3 := \langle A_3; \neg, \wedge_{OL}, \vee_{OL}, \rightarrow_{OL} \rangle$ .
- *Farrell's logic*  $F$ , induced by  $\langle \mathbf{F}_3, \{1/2, 1\} \rangle$ , with  $\mathbf{F}_3 := \langle A_3; \neg, \wedge_K, \vee_K, \rightarrow_F \rangle$ .

## 2. The three-valued case

Let  $A_3 := \{0, 1/2, 1\}$ . Our three-valued logics are:

- *De Finetti's logic* DF, induced by  $\langle \mathbf{DF}_3, \{1/2, 1\} \rangle$ , with  $\mathbf{DF}_3 := \langle A_3; \neg, \wedge_K, \vee_K, \rightarrow_{DF} \rangle$ .
- *Cooper's logic* OL, induced by  $\langle \mathbf{OL}_3, \{1/2, 1\} \rangle$ , with  $\mathbf{OL}_3 := \langle A_3; \neg, \wedge_{OL}, \vee_{OL}, \rightarrow_{OL} \rangle$ .
- *Farrell's logic* F, induced by  $\langle \mathbf{F}_3, \{1/2, 1\} \rangle$ , with  $\mathbf{F}_3 := \langle A_3; \neg, \wedge_K, \vee_K, \rightarrow_F \rangle$ .
- *Cantwell's logic* CN, induced by  $\langle \mathbf{CN}_3, \{1/2, 1\} \rangle$ , with  $\mathbf{CN}_3 := \langle A_3; \neg, \wedge_K, \vee_K, \rightarrow_{OL} \rangle$ .



### 3. Twist structures

### 3. Twist structures

Idea: to obtain semantics for the target logics by means of constructions in terms of already known algebras (*twist structures*).

### 3. Twist structures

Idea: to obtain semantics for the target logics by means of constructions in terms of already known algebras (*twist structures*).

- First, define some class of algebras associated with the logic.

### 3. Twist structures

Idea: to obtain semantics for the target logics by means of constructions in terms of already known algebras (*twist structures*).

- First, define some class of algebras associated with the logic.
- Then, check that every twist structure belongs to this class.

### 3. Twist structures

Idea: to obtain semantics for the target logics by means of constructions in terms of already known algebras (*twist structures*).

- First, define some class of algebras associated with the logic.
- Then, check that every twist structure belongs to this class.
- Finally, prove the *twist representation result*, i.e., that every algebra from the original class is isomorphic to some twist structure.

### 3. Twist structures

Idea: to obtain semantics for the target logics by means of constructions in terms of already known algebras (*twist structures*).

- First, define some class of algebras associated with the logic.
- Then, check that every twist structure belongs to this class.
- Finally, prove the *twist representation result*, i.e., that every algebra from the original class is isomorphic to some twist structure.

These results can be achieved for DF, OL, F and CN.

### 3. Twist structures

Idea: to obtain semantics for the target logics by means of constructions in terms of already known algebras (*twist structures*).

- First, define some class of algebras associated with the logic.
- Then, check that every twist structure belongs to this class.
- Finally, prove the *twist representation result*, i.e., that every algebra from the original class is isomorphic to some twist structure.

These results can be achieved for DF, OL, F and CN.

In short, we wish to identify:

$$\mathbf{0} \mapsto (0, 1), \quad \mathbf{1/2} \mapsto (1, 1), \quad \mathbf{1} \mapsto (1, 0).$$

## 4. The four-valued case



## 4. The four-valued case

Suppose that our factor algebras behave in a Boolean way. Then, the connectives look as follows:

## 4. The four-valued case

Suppose that our factor algebras behave in a Boolean way. Then, the connectives look as follows:

$$- \neg(x, y) := (y, x),$$

## 4. The four-valued case

Suppose that our factor algebras behave in a Boolean way. Then, the connectives look as follows:

- $\neg(x, y) := (y, x),$
- $(x_1, y_1) \wedge_K (x_2, y_2) := (x_1 \wedge x_2, y_1 \vee y_2),$

## 4. The four-valued case

Suppose that our factor algebras behave in a Boolean way. Then, the connectives look as follows:

- $\neg(x, y) := (y, x),$
- $(x_1, y_1) \wedge_K (x_2, y_2) := (x_1 \wedge x_2, y_1 \vee y_2),$
- $(x_1, y_1) \wedge_{OL} (x_2, y_2) := (x_1 \wedge x_2, (x_1 \rightarrow y_2) \wedge (x_2 \rightarrow y_1)),$

## 4. The four-valued case

Suppose that our factor algebras behave in a Boolean way. Then, the connectives look as follows:

- $\neg(x, y) := (y, x),$
- $(x_1, y_1) \wedge_K (x_2, y_2) := (x_1 \wedge x_2, y_1 \vee y_2),$
- $(x_1, y_1) \wedge_{OL} (x_2, y_2) := (x_1 \wedge x_2, (x_1 \rightarrow y_2) \wedge (x_2 \rightarrow y_1)),$
- $(x_1, y_1) \rightarrow_{DF} (x_2, y_2) = (y_1 \vee (x_1 \wedge x_2), y_1 \vee y_2),$

## 4. The four-valued case

Suppose that our factor algebras behave in a Boolean way. Then, the connectives look as follows:

- $\neg(x, y) := (y, x),$
- $(x_1, y_1) \wedge_K (x_2, y_2) := (x_1 \wedge x_2, y_1 \vee y_2),$
- $(x_1, y_1) \wedge_{OL} (x_2, y_2) := (x_1 \wedge x_2, (x_1 \rightarrow y_2) \wedge (x_2 \rightarrow y_1)),$
- $(x_1, y_1) \rightarrow_{DF} (x_2, y_2) = (y_1 \vee (x_1 \wedge x_2), y_1 \vee y_2),$
- $(x_1, y_1) \rightarrow_{OL} (x_2, y_2) := (x_1 \rightarrow x_2, x_1 \rightarrow y_2),$

## 4. The four-valued case

Suppose that our factor algebras behave in a Boolean way. Then, the connectives look as follows:

- $\neg(x, y) := (y, x),$
- $(x_1, y_1) \wedge_K (x_2, y_2) := (x_1 \wedge x_2, y_1 \vee y_2),$
- $(x_1, y_1) \wedge_{OL} (x_2, y_2) := (x_1 \wedge x_2, (x_1 \rightarrow y_2) \wedge (x_2 \rightarrow y_1)),$
- $(x_1, y_1) \rightarrow_{DF} (x_2, y_2) = (y_1 \vee (x_1 \wedge x_2), y_1 \vee y_2),$
- $(x_1, y_1) \rightarrow_{OL} (x_2, y_2) := (x_1 \rightarrow x_2, x_1 \rightarrow y_2),$
- $(x_1, y_1) \rightarrow_F (x_2, y_2) := (x_1 \rightarrow x_2, y_1 \vee y_2).$

## 4. The four-valued case

Suppose that our factor algebras behave in a Boolean way. Then, the connectives look as follows:

- $\neg(x, y) := (y, x),$
- $(x_1, y_1) \wedge_K (x_2, y_2) := (x_1 \wedge x_2, y_1 \vee y_2),$
- $(x_1, y_1) \wedge_{OL} (x_2, y_2) := (x_1 \wedge x_2, (x_1 \rightarrow y_2) \wedge (x_2 \rightarrow y_1)),$
- $(x_1, y_1) \rightarrow_{DF} (x_2, y_2) = (y_1 \vee (x_1 \wedge x_2), y_1 \vee y_2),$
- $(x_1, y_1) \rightarrow_{OL} (x_2, y_2) := (x_1 \rightarrow x_2, x_1 \rightarrow y_2),$
- $(x_1, y_1) \rightarrow_F (x_2, y_2) := (x_1 \rightarrow x_2, y_1 \vee y_2).$

Let us denote  $\top := 1/2$  in what follows.



## 4. The four-valued case

Suppose that our factor algebras behave in a Boolean way. Then, the connectives look as follows:

- $\neg(x, y) := (y, x),$
- $(x_1, y_1) \wedge_K (x_2, y_2) := (x_1 \wedge x_2, y_1 \vee y_2),$
- $(x_1, y_1) \wedge_{OL} (x_2, y_2) := (x_1 \wedge x_2, (x_1 \rightarrow y_2) \wedge (x_2 \rightarrow y_1)),$
- $(x_1, y_1) \rightarrow_{DF} (x_2, y_2) = (y_1 \vee (x_1 \wedge x_2), y_1 \vee y_2),$
- $(x_1, y_1) \rightarrow_{OL} (x_2, y_2) := (x_1 \rightarrow x_2, x_1 \rightarrow y_2),$
- $(x_1, y_1) \rightarrow_F (x_2, y_2) := (x_1 \rightarrow x_2, y_1 \vee y_2).$

Let us denote  $\top := 1/2$  in what follows. What if we send:

$$\perp \mapsto (0, 0)$$

and compute the tables?

## 4.1. Adding a semantic gap

## 4.1. Adding a semantic gap

The tables look as follows:

$\rightarrow_{DF}$	<b>0</b>	$\perp$	<b>T</b>	<b>1</b>
<b>0</b>	<b>T</b>	<b>T</b>	<b>T</b>	<b>T</b>
$\perp$	<b>0</b>	$\perp$	<b>0</b>	$\perp$
<b>T</b>	<b>T</b>	<b>T</b>	<b>T</b>	<b>T</b>
<b>1</b>	<b>0</b>	$\perp$	<b>T</b>	<b>1</b>

$\rightarrow_{OL}$	<b>0</b>	$\perp$	<b>T</b>	<b>1</b>
<b>0</b>	<b>T</b>	<b>T</b>	<b>T</b>	<b>T</b>
$\perp$	<b>T</b>	<b>T</b>	<b>T</b>	<b>T</b>
<b>T</b>	<b>0</b>	$\perp$	<b>T</b>	<b>1</b>
<b>1</b>	<b>0</b>	$\perp$	<b>T</b>	<b>1</b>

$\rightarrow_F$	<b>0</b>	$\perp$	<b>T</b>	<b>1</b>
<b>0</b>	<b>T</b>	<b>T</b>	<b>T</b>	<b>T</b>
$\perp$	<b>T</b>	<b>1</b>	<b>T</b>	<b>1</b>
<b>T</b>	<b>0</b>	<b>0</b>	<b>T</b>	<b>T</b>
<b>1</b>	<b>0</b>	$\perp$	<b>T</b>	<b>1</b>

## 4.1. Adding a semantic gap

The tables look as follows:

$\rightarrow_{DF}$	0	$\perp$	T	1
0	T	T	T	T
$\perp$	0	$\perp$	0	$\perp$
T	T	T	T	T
1	0	$\perp$	T	1

$\rightarrow_{OL}$	0	$\perp$	T	1
0	T	T	T	T
$\perp$	T	T	T	T
T	0	$\perp$	T	1
1	0	$\perp$	T	1

$\rightarrow_F$	0	$\perp$	T	1
0	T	T	T	T
$\perp$	T	1	T	1
T	0	0	T	T
1	0	$\perp$	T	1

In addition,

	$\neg$	$\wedge_K$	0	$\perp$	T	1
0	1	0	0	0	0	0
$\perp$	$\perp$	$\perp$	0	T	0	T
T	T	T	0	0	T	T
1	0	1	0	$\perp$	T	1

	$\wedge_{OL}$	0	$\perp$	T	1
0	0	0	0	0	0
$\perp$	0	0	$\perp$	$\perp$	$\perp$
T	0	$\perp$	T	1	1
1	0	$\perp$	1	1	1

Where one sets

$$x \vee_K y := \neg(\neg x \wedge_K \neg y),$$

$$x \vee_{OL} y := \neg(\neg x \wedge_{OL} \neg y).$$

## 4.1. Adding a semantic gap

## 4.1. Adding a semantic gap

Let  $A_4 := \{\mathbf{0}, \perp, \top, \mathbf{1}\}$ . Our four-valued logics are:

## 4.1. Adding a semantic gap

Let  $A_4 := \{\mathbf{0}, \perp, \top, \mathbf{1}\}$ . Our four-valued logics are:

- DFg, induced by  $\langle \mathbf{DFg}, \{\top, \mathbf{1}\} \rangle$ , with  $\mathbf{DFg} := \langle A_4; \neg, \wedge_K, \vee_K, \rightarrow_{DF} \rangle$ .

## 4.1. Adding a semantic gap

Let  $A_4 := \{\mathbf{0}, \perp, \top, \mathbf{1}\}$ . Our four-valued logics are:

- DFg, induced by  $\langle \mathbf{DFg}, \{\top, \mathbf{1}\} \rangle$ , with  $\mathbf{DFg} := \langle A_4; \neg, \wedge_K, \vee_K, \rightarrow_{DF} \rangle$ .
- OLg, induced by  $\langle \mathbf{OLg}, \{\top, \mathbf{1}\} \rangle$ , with  $\mathbf{OLg} := \langle A_4; \neg, \wedge_{OL}, \vee_{OL}, \rightarrow_{OL} \rangle$ .



## 4.1. Adding a semantic gap

Let  $A_4 := \{\mathbf{0}, \perp, \top, \mathbf{1}\}$ . Our four-valued logics are:

- DFg, induced by  $\langle \mathbf{DFg}, \{\top, \mathbf{1}\} \rangle$ , with  $\mathbf{DFg} := \langle A_4; \neg, \wedge_K, \vee_K, \rightarrow_{DF} \rangle$ .
- OLg, induced by  $\langle \mathbf{OLg}, \{\top, \mathbf{1}\} \rangle$ , with  $\mathbf{OLg} := \langle A_4; \neg, \wedge_{OL}, \vee_{OL}, \rightarrow_{OL} \rangle$ .
- Fg, induced by  $\langle \mathbf{Fg}, \{\top, \mathbf{1}\} \rangle$ , with  $\mathbf{Fg} := \langle A_4; \neg, \wedge_K, \vee_K, \rightarrow_F \rangle$ .

## 4.1. Adding a semantic gap

Let  $A_4 := \{\mathbf{0}, \perp, \top, \mathbf{1}\}$ . Our four-valued logics are:

- DFg, induced by  $\langle \mathbf{DFg}, \{\top, \mathbf{1}\} \rangle$ , with  $\mathbf{DFg} := \langle A_4; \neg, \wedge_K, \vee_K, \rightarrow_{DF} \rangle$ .
- OLg, induced by  $\langle \mathbf{OLg}, \{\top, \mathbf{1}\} \rangle$ , with  $\mathbf{OLg} := \langle A_4; \neg, \wedge_{OL}, \vee_{OL}, \rightarrow_{OL} \rangle$ .
- Fg, induced by  $\langle \mathbf{Fg}, \{\top, \mathbf{1}\} \rangle$ , with  $\mathbf{Fg} := \langle A_4; \neg, \wedge_K, \vee_K, \rightarrow_F \rangle$ .
- CNg, induced by  $\langle \mathbf{CNg}, \{\top, \mathbf{1}\} \rangle$ , with  $\mathbf{CNg} := \langle A_4; \neg, \wedge_K, \vee_K, \rightarrow_{OL} \rangle$ .

## 4.1. Adding a semantic gap

Let  $A_4 := \{0, \perp, \top, 1\}$ . Our four-valued logics are:

- DFg, induced by  $\langle \mathbf{DFg}, \{\top, 1\} \rangle$ , with  $\mathbf{DFg} := \langle A_4; \neg, \wedge_K, \vee_K, \rightarrow_{DF} \rangle$ .
- OLg, induced by  $\langle \mathbf{OLg}, \{\top, 1\} \rangle$ , with  $\mathbf{OLg} := \langle A_4; \neg, \wedge_{OL}, \vee_{OL}, \rightarrow_{OL} \rangle$ .
- Fg, induced by  $\langle \mathbf{Fg}, \{\top, 1\} \rangle$ , with  $\mathbf{Fg} := \langle A_4; \neg, \wedge_K, \vee_K, \rightarrow_F \rangle$ .
- CNg, induced by  $\langle \mathbf{CNg}, \{\top, 1\} \rangle$ , with  $\mathbf{CNg} := \langle A_4; \neg, \wedge_K, \vee_K, \rightarrow_{OL} \rangle$ .

Then, it turns out that one can prove twist representation results for DFg, CNg and Fg.

## 4.2. Adding a falsity

## 4.2. Adding a falsity

In the previous approach, one could see  $\top$  and  $\perp$  as corresponding to semantic *gluts* and *gaps*, respectively.

## 4.2. Adding a falsity

In the previous approach, one could see  $\top$  and  $\perp$  as corresponding to semantic *gluts* and *gaps*, respectively.

However, one could see  $\top$  and  $\perp$  as representing *vacuously true* and *vacuously false* statements.

## 4.2. Adding a falsity

In the previous approach, one could see  $\top$  and  $\perp$  as corresponding to semantic *gluts* and *gaps*, respectively.

However, one could see  $\top$  and  $\perp$  as representing *vacuously true* and *vacuously false* statements.

This entails a different behavior with respect to negation.

## 4.2. Adding a falsity

In the previous approach, one could see  $\top$  and  $\perp$  as corresponding to semantic *gluts* and *gaps*, respectively.

However, one could see  $\top$  and  $\perp$  as representing *vacuously true* and *vacuously false* statements.

This entails a different behavior with respect to negation. We wish to define:

$$\neg(x, y) := (\neg x, \neg y).$$



## 4.2. Adding a falsity

In the previous approach, one could see  $\top$  and  $\perp$  as corresponding to semantic *gluts* and *gaps*, respectively.

However, one could see  $\top$  and  $\perp$  as representing *vacuously true* and *vacuously false* statements.

This entails a different behavior with respect to negation. We wish to define:

$$\neg(x, y) := (\neg x, \neg y).$$

Hence, we extend the tables above with:

	$\neg$
<b>0</b>	<b>1</b>
$\perp$	$\top$
$\top$	$\perp$
<b>1</b>	<b>0</b>

## 4.2. Adding a falsity

## 4.2. Adding a falsity

Let  $A_4 := \{\mathbf{0}, \perp, \top, \mathbf{1}\}$ . Accordingly, we can define:

## 4.2. Adding a falsity

Let  $A_4 := \{\mathbf{0}, \perp, \top, \mathbf{1}\}$ . Accordingly, we can define:

- $\text{DFf}^-$ , induced by  $\langle \mathbf{DFf}^-, \{\top, \mathbf{1}\} \rangle$ , with  $\mathbf{DFf}^- := \langle A_4; -, \wedge_K, \vee_K, \top \rangle$ .

## 4.2. Adding a falsity

Let  $A_4 := \{\mathbf{0}, \perp, \top, \mathbf{1}\}$ . Accordingly, we can define:

- $\text{DFf}^-$ , induced by  $\langle \mathbf{DFf}^-, \{\top, \mathbf{1}\} \rangle$ , with  $\mathbf{DFf}^- := \langle A_4; -, \wedge_K, \vee_K, \top \rangle$ .
- $\text{DFf}$ , induced by  $\langle \mathbf{DFf}, \{\top, \mathbf{1}\} \rangle$ , with  $\mathbf{DFf} := \langle A_4; -, \wedge_K, \vee_K, \rightarrow_{\text{DF}} \rangle$ .

## 4.2. Adding a falsity

Let  $A_4 := \{\mathbf{0}, \perp, \top, \mathbf{1}\}$ . Accordingly, we can define:

- $\text{DFf}^-$ , induced by  $\langle \mathbf{DFf}^-, \{\top, \mathbf{1}\} \rangle$ , with  $\mathbf{DFf}^- := \langle A_4; -, \wedge_K, \vee_K, \top \rangle$ .
- $\text{DFf}$ , induced by  $\langle \mathbf{DFf}, \{\top, \mathbf{1}\} \rangle$ , with  $\mathbf{DFf} := \langle A_4; -, \wedge_K, \vee_K, \rightarrow_{\text{DF}} \rangle$ .
- $\text{OLf}$ , induced by  $\langle \mathbf{OLf}, \{\top, \mathbf{1}\} \rangle$ , with  $\mathbf{OLf} := \langle A_4; -, \wedge_{\text{OL}}, \vee_{\text{OL}}, \rightarrow_{\text{OL}} \rangle$ .

## 4.2. Adding a falsity

Let  $A_4 := \{\mathbf{0}, \perp, \top, \mathbf{1}\}$ . Accordingly, we can define:

- $\text{DFf}^-$ , induced by  $\langle \mathbf{DFf}^-, \{\top, \mathbf{1}\} \rangle$ , with  $\mathbf{DFf}^- := \langle A_4; -, \wedge_K, \vee_K, \top \rangle$ .
- $\text{DFf}$ , induced by  $\langle \mathbf{DFf}, \{\top, \mathbf{1}\} \rangle$ , with  $\mathbf{DFf} := \langle A_4; -, \wedge_K, \vee_K, \rightarrow_{\text{DF}} \rangle$ .
- $\text{OLf}$ , induced by  $\langle \mathbf{OLf}, \{\top, \mathbf{1}\} \rangle$ , with  $\mathbf{OLf} := \langle A_4; -, \wedge_{\text{OL}}, \vee_{\text{OL}}, \rightarrow_{\text{OL}} \rangle$ .
- $\text{Ff}$ , induced by  $\langle \mathbf{Ff}, \{\top, \mathbf{1}\} \rangle$ , with  $\mathbf{Ff} := \langle A_4; -, \wedge_K, \vee_K, \rightarrow_{\text{F}} \rangle$ .

## 4.2. Adding a falsity

Let  $A_4 := \{\mathbf{0}, \perp, \top, \mathbf{1}\}$ . Accordingly, we can define:

- $\text{DFf}^-$ , induced by  $\langle \mathbf{DFf}^-, \{\top, \mathbf{1}\} \rangle$ , with  $\mathbf{DFf}^- := \langle A_4; -, \wedge_K, \vee_K, \top \rangle$ .
- $\text{DFf}$ , induced by  $\langle \mathbf{DFf}, \{\top, \mathbf{1}\} \rangle$ , with  $\mathbf{DFf} := \langle A_4; -, \wedge_K, \vee_K, \rightarrow_{\text{DF}} \rangle$ .
- $\text{OLf}$ , induced by  $\langle \mathbf{OLf}, \{\top, \mathbf{1}\} \rangle$ , with  $\mathbf{OLf} := \langle A_4; -, \wedge_{\text{OL}}, \vee_{\text{OL}}, \rightarrow_{\text{OL}} \rangle$ .
- $\text{Ff}$ , induced by  $\langle \mathbf{Ff}, \{\top, \mathbf{1}\} \rangle$ , with  $\mathbf{Ff} := \langle A_4; -, \wedge_K, \vee_K, \rightarrow_{\text{F}} \rangle$ .
- $\text{CNf}$ , induced by  $\langle \mathbf{CNf}, \{\top, \mathbf{1}\} \rangle$ , with  $\mathbf{CNf} := \langle A_4; -, \wedge_K, \vee_K, \rightarrow_{\text{OL}} \rangle$ .



## 4.2. Adding a falsity

Let  $A_4 := \{\mathbf{0}, \perp, \top, \mathbf{1}\}$ . Accordingly, we can define:

- $\text{DFf}^-$ , induced by  $\langle \mathbf{DFf}^-, \{\top, \mathbf{1}\} \rangle$ , with  $\mathbf{DFf}^- := \langle A_4; -, \wedge_K, \vee_K, \top \rangle$ .
- $\text{DFf}$ , induced by  $\langle \mathbf{DFf}, \{\top, \mathbf{1}\} \rangle$ , with  $\mathbf{DFf} := \langle A_4; -, \wedge_K, \vee_K, \rightarrow_{\text{DF}} \rangle$ .
- $\text{OLf}$ , induced by  $\langle \mathbf{OLf}, \{\top, \mathbf{1}\} \rangle$ , with  $\mathbf{OLf} := \langle A_4; -, \wedge_{\text{OL}}, \vee_{\text{OL}}, \rightarrow_{\text{OL}} \rangle$ .
- $\text{Ff}$ , induced by  $\langle \mathbf{Ff}, \{\top, \mathbf{1}\} \rangle$ , with  $\mathbf{Ff} := \langle A_4; -, \wedge_K, \vee_K, \rightarrow_{\text{F}} \rangle$ .
- $\text{CNf}$ , induced by  $\langle \mathbf{CNf}, \{\top, \mathbf{1}\} \rangle$ , with  $\mathbf{CNf} := \langle A_4; -, \wedge_K, \vee_K, \rightarrow_{\text{OL}} \rangle$ .

Then, one can prove twist representation results for  $\text{DFf}^-$  and  $\text{Ff}$ .

## 5. Further work

## 5. Further work

- i. Study the cases of OLg, OLf, DFF and CNf.

## 5. Further work

- i. Study the cases of OLg, OLf, DFF and CNf.
- ii. Study the implications of the twist representation results.

## 5. Further work

- i. Study the cases of OLg, OLf, DFF and CNf.
- ii. Study the implications of the twist representation results.
- iii. Study algebraizability and axiomatizability issues regarding the new logics.

## 5. Further work

- i. Study the cases of OLg, OLf, DFF and CNf.
- ii. Study the implications of the twist representation results.
- iii. Study algebraizability and axiomatizability issues regarding the new logics.
- iv. Provide a more systematic philosophical account for the new logics.

# Bibliography



Cantwell, J. (2008)

*The logic of conditional negation.*

Notre Dame Journal of Formal Logic 49(3): 245-260.



Cooper, W.S. (1968)

*The Propositional Logic of Ordinary Discourse.*

Inquiry: An Interdisciplinary Journal of Philosophy 11(1-4), 295–320.



Egré, P., Rossi, L. & Sprenger, J. (2021)

*De Finettian logics of indicative conditionals part I: trivalent semantics and validity.*

Journal of Philosophical Logic 50(2), 187–213.



Farrell, R.J. (1986)

*Implication and presupposition.*

Notre Dame Journal of Formal Logic, Volume 27, Number 1.



Greati, V., Marcelino, S. & Rieviccio, U. (2025)

*Axiomatizing the Logic of Ordinary Discourse.*

Proceedings of IPMU 2024, 390–405.

## Bibliography



Greati, V., Marcelino, S., Riviello, U. & Muñoz Pérez, M. (2026)

*Analytic calculi for logics of indicative conditionals.*

In: Pozzato, G. L., Uustalu, T. (eds) Automated Reasoning with Analytic Tableaux and Related Methods. TABLEUX 2025. Lecture Notes in Computer Science(), vol 15980. Springer, Cham.



de Finetti, B. (1936)

*La logique de la probabilité.*

Actes du Congrès International de Philosophie Scientifique.



Muñoz Pérez, M. & Riviuccio, U. (2025)

*Indicative conditionals: Some algebraic considerations.*

In Kozen, D. & de Queiroz, R. (eds) Logic, Language, Information, and Computation, WoLLIC 2025, Lecture Notes in Computer Science, vol. 15942, Springer



Muñoz Pérez, M. (2025)

### Four-valued logics of indicative conditionals.

Preprint, available at arXiv.org.



Rivieccio, U. (2025)

*The algebra of ordinary discourse. On the semantics of Cooper's logic.*

Archive for Mathematical Logic.